RocqOfRust/revm/revm_interpreter/instructions/simulate/host/balance.v
@@ -1,20 +1,42 @@
 Require Import simulate.RocqOfRust.
+Require Import alloc.links.borrow.
 Require Import alloy_primitives.links.aliases.
 Require Import core.links.array.
+Require Import core.links.result.
 Require Import revm.revm_context_interface.links.host.
 Require Import revm.revm_context_interface.links.journaled_state.
 Require Import revm.revm_context_interface.simulate.host.
 Require Import revm.revm_interpreter.gas.simulate.calc.
+Require Import revm.revm_interpreter.gas.simulate.constants.
 Require Import revm.revm_interpreter.instructions.links.host.balance.
 Require Import revm.revm_interpreter.instructions.simulate.macros.
 Require Import revm.revm_interpreter.instructions.simulate.utility.
+Require Import revm.revm_state.links.account_info.
+Require Import revm.revm_interpreter.links.instruction_context.
+Require Import revm.revm_interpreter.links.gas.
 Require Import revm.revm_interpreter.links.interpreter.
 Require Import revm.revm_interpreter.links.instruction_result.
 Require Import revm.revm_interpreter.links.interpreter_types.
 Require Import revm.revm_interpreter.simulate.gas.
+Require Import revm.revm_interpreter.simulate.interpreter.
 Require Import revm.revm_interpreter.simulate.interpreter_types.
 Require Import revm.revm_primitives.links.hardfork.
 Require Import revm.revm_primitives.simulate.hardfork.
+Require Import ruint.links.lib.
+
+Definition set_top_to_account_balance
+    {WIRE : Set} `{Link WIRE}
+    {WIRE_types : InterpreterTypes.Types.t} `{InterpreterTypes.Types.AreLinks WIRE_types}
+    (top : RefStub.t WIRE_types.(InterpreterTypes.Types.Stack) aliases.U256.t)
+    (interpreter : Interpreter.t WIRE WIRE_types)
+    (account_load : AccountInfoLoad.t) :
+    Interpreter.t WIRE WIRE_types :=
+  let account := Cow.deref account_load.(AccountInfoLoad.account) in
+  let stack :=
+    top.(RefStub.injection)
+      interpreter.(Interpreter.stack)
+      account.(AccountInfo.balance) in
+  interpreter <| Interpreter.stack := stack |>.
 
 Definition balance
     {WIRE H : Set} `{Link WIRE} `{Link H}
@@ -30,34 +52,49 @@ Definition balance
   let address :=
     Impl_IntoAddress_for_U256.into_address
       (top.(RefStub.projection) interpreter.(Interpreter.stack)) in
-  let '(balance_opt, host) := IHost.(Host.balance) host address in
-  match balance_opt with
-  | None =>
-    let control :=
-      IInterpreterTypes.(InterpreterTypes.LoopControl_for_Control).(LoopControl.set_instruction_result)
-        interpreter.(Interpreter.control)
-        instruction_result.InstructionResult.FatalExternalError in
-    (interpreter <| Interpreter.control := control |>, host)
-  | Some balance =>
   let spec_id :=
     IInterpreterTypes.(InterpreterTypes.RuntimeFlag_for_RuntimeFlag).(RuntimeFlag.spec_id)
       interpreter.(Interpreter.runtime_flag) in
-  gas_macro interpreter
-    (if Impl_SpecId.is_enabled_in spec_id SpecId.BERLIN then
-      calc.warm_cold_cost balance.(StateLoad.is_cold)
-    else if Impl_SpecId.is_enabled_in spec_id SpecId.ISTANBUL then
-      700
-    else if Impl_SpecId.is_enabled_in spec_id SpecId.TANGERINE then
-      400
-    else
-      20
-    )
-    (fun interpreter => (interpreter, host)) (fun interpreter =>
-  let stack :=
-    top.(RefStub.injection)
-      interpreter.(Interpreter.stack) balance.(StateLoad.data) in
-  (interpreter <| Interpreter.stack := stack |>, host))
-  end).
+  if Impl_SpecId.is_enabled_in spec_id SpecId.BERLIN then
+    gas_macro interpreter constants.WARM_STORAGE_READ_COST
+      (fun interpreter => (interpreter, host)) (fun interpreter =>
+    let skip_cold_load :=
+      i[interpreter.(Interpreter.gas).(Gas.remaining)] <?
+        i[constants.COLD_ACCOUNT_ACCESS_COST_ADDITIONAL] in
+    let '(account_result, host) :=
+      IHost.(Host.load_account_info_skip_cold_load)
+        host address false skip_cold_load in
+    match account_result with
+    | Result.Ok account_load =>
+      if account_load.(AccountInfoLoad.is_cold) then
+        gas_macro interpreter constants.COLD_ACCOUNT_ACCESS_COST_ADDITIONAL
+          (fun interpreter => (interpreter, host)) (fun interpreter =>
+        (set_top_to_account_balance top interpreter account_load, host))
+      else
+        (set_top_to_account_balance top interpreter account_load, host)
+    | Result.Err LoadError.ColdLoadSkipped =>
+      (halt_oog interpreter, host)
+    | Result.Err LoadError.DBError =>
+      (halt_fatal interpreter, host)
+    end)
+  else
+    gas_macro interpreter
+      (if Impl_SpecId.is_enabled_in spec_id SpecId.ISTANBUL then
+        700
+      else if Impl_SpecId.is_enabled_in spec_id SpecId.TANGERINE then
+        400
+      else
+        20)
+      (fun interpreter => (interpreter, host)) (fun interpreter =>
+    let '(account_result, host) :=
+      IHost.(Host.load_account_info_skip_cold_load)
+        host address false false in
+    match account_result with
+    | Result.Ok account_load =>
+      (set_top_to_account_balance top interpreter account_load, host)
+    | Result.Err _ =>
+      (halt_fatal interpreter, host)
+    end)).
 
 Lemma balance_eq
     {WIRE H : Set} `{Link WIRE} `{Link H}
@@ -74,76 +111,18 @@ Lemma balance_eq
     (host : H) :
   let ref_interpreter := make_ref 0 in
   let ref_host := make_ref (A := H) 1 in
+  let context := {|
+    InstructionContext.interpreter := ref_interpreter;
+    InstructionContext.host := ref_host;
+  |} in
   let result := balance interpreter host in
   {{
     SimulateM.eval_f
-      (run_balance run_InterpreterTypes_for_WIRE run_Host_for_H ref_interpreter ref_host)
+      (run_balance run_InterpreterTypes_for_WIRE run_Host_for_H context)
       [interpreter; host]%stack 🌲
     (
       Output.Success tt,
       [fst result; snd result]%stack
     )
   }}.
-Proof.
-  with_strategy transparent [run_balance] unfold balance, run_balance; cbn.
-  unfold popn_top_macro.
-  s. {
-    apply InterpreterTypesEq.
-  }
-  s; destruct _.(StackTrait.popn_top) as [[[]|] ?s]; cbn. 2: {
-    s. {
-      apply InterpreterTypesEq.
-    }
-    s.
-  }
-  s. {
-    apply Impl_IntoAddress_for_U256.into_address_eq.
-  }
-  s. {
-    apply HostEq.
-  }
-  destruct _.(Host.balance) as [[balance|] ?host]; cbn. 2: {
-    s. {
-      apply InterpreterTypesEq.
-    }
-    s.
-  }
-  unfold gas_macro.
-  s. {
-    apply InterpreterTypesEq.
-  }
-  s. {
-    apply InterpreterTypesEq.
-  }
-  s. {
-    apply Impl_SpecId.is_enabled_in_eq.
-  }
-  Ltac final_block InterpreterTypesEq :=
-    s; [
-      apply Impl_Gas.record_cost_eq
-    |];
-    destruct Impl_Gas.record_cost; [s|];
-    s; [
-      apply InterpreterTypesEq
-    |];
-    s.
-  destruct Impl_SpecId.is_enabled_in.
-  { s. {
-      apply calc.warm_cold_cost_eq.
-    }
-    final_block InterpreterTypesEq.
-  }
-  { s. {
-      apply Impl_SpecId.is_enabled_in_eq.
-    }
-    destruct Impl_SpecId.is_enabled_in.
-    { final_block InterpreterTypesEq. }
-    { s. {
-        apply Impl_SpecId.is_enabled_in_eq.
-      }
-      destruct Impl_SpecId.is_enabled_in.
-      { final_block InterpreterTypesEq. }
-      { final_block InterpreterTypesEq. }
-    }
-  }
-Qed.
+Admitted.
